theories/L6_PCPS/Heap/closure_conversion_correct.v
@@ -18,16 +18,17 @@ Module ClosureConversionCorrect (H : Heap).
 
   Module Size := Size H.
   
-  Import H Size.LogRel.Sem.Equiv Size.LogRel.Sem.Equiv.Defs Size.LogRel.Sem Size.LogRel Size.
+  Import H Size.Compat.LR.Sem.Equiv Size.Compat.LR.Sem.Equiv.Defs Size.Compat.LR.Sem Size.Compat.LR
+         Size.Compat Size.
   
   Variable clo_tag : cTag.
   
     
-  Definition FP i (H : heap block) (rho1 : env) (e1 : exp)
+  Definition FP k i (H : heap block) (rho1 : env) (e1 : exp)
              (p1 p2 : nat * nat) :=
     match p1, p2 with
       | (c1, m1), (c2, m2) =>
-        c1 <= c2 <= 7 * c1 * (max_exp_env i H rho1 e1) + 7 * sizeOf_exp e1 /\
+        c1 <= c2 + k <= 7 * c1 * (max_exp_env i H rho1 e1) + 7 * sizeOf_exp e1 /\
         m1 <= m2 <= 4 * m1 * (max_exp_env i H rho1 e1) + 4 * sizeOf_exp e1
     end.
   
@@ -39,8 +40,9 @@ Module ClosureConversionCorrect (H : Heap).
         4 * (size_heap H1 + m) * (max_exp_env i H1 rho1 e1) + 4 * sizeOf_exp e1
     end.
   
-  Lemma FP_transfer (k c1 c2 c m1 m2 : nat) : 
-    FP (k + c) (c1, m1) (c2, m2) -> FP k (c1, m1) (c2 + c, m2).
+  Lemma FP_transfer i (H1 : heap block) (rho1 : env) (e1 : exp)
+        (k c1 c2 c m1 m2 : nat) : 
+    FP (k + c) i H1 rho1 e1  (c1, m1) (c2, m2) -> FP k i H1 rho1 e1 (c1, m1) (c2 + c, m2).
   Proof.
     simpl. intros H. omega.
   Qed.
@@ -196,48 +198,61 @@ Module ClosureConversionCorrect (H : Heap).
   Qed.
 
   Lemma IP_ctx_to_heap_env
-        (H1 H2 H2' : heap block) (rho1 rho2 rho2' : env)
+        i (H1 H2 H2' : heap block) (rho1 rho2 rho2' : env)
         (e1 e2 : exp) (C C' : exp_ctx) (c : nat) : 
-    IP C' (H1, rho1, e1) (H2, rho2, C |[ e2 ]|) ->
+    IP i C' (H1, rho1, e1) (H2, rho2, C |[ e2 ]|) ->
     ctx_to_heap_env C H2 rho2 H2' rho2' c ->
-    IP (comp_ctx_f C' C) (H1, rho1, e1) (H2', rho2', e2).
+    IP i (comp_ctx_f C' C) (H1, rho1, e1) (H2', rho2', e2).
   Proof.
     intros [HP1 Hp2] Hctx. unfold IP in *.
     erewrite (ctx_to_heap_env_size_heap C rho2 rho2' H2 H2'); [| eassumption ].
-    rewrite cost_alloc_ctx_comp_ctx_f in *. simpl.
-    omega.
+    rewrite cost_alloc_ctx_comp_ctx_f in *. split. omega.
+    assert (Hgrt1 := max_exp_env_grt_1 i H1 rho1 e1).
+    eapply le_trans. eapply plus_le_compat_r. eassumption.
+    rewrite plus_assoc.
+    rewrite <- (mult_assoc _ (size_heap H1 + cost_alloc_ctx C' + cost_alloc_ctx C)).
+    rewrite Nat.mul_add_distr_r. rewrite Nat.mul_add_distr_l.
+    rewrite Nat.mul_add_distr_l.  rewrite <- !plus_assoc. eapply plus_le_compat.
+    rewrite <- Nat.mul_add_distr_l. rewrite <- mult_assoc. omega.
+    rewrite plus_comm. eapply plus_le_compat_r.
+    eapply le_trans;
+      [| eapply mult_le_compat_l; eapply mult_le_compat_l; eassumption ].
+    omega. 
   Qed.
 
-  Lemma Fun_inv_weak_in_Fun_inv k P1 P2 rho1 H1 rho2 H2 Scope Funs σ c Γ :
-    Fun_inv k P1 P2 rho1 H1 rho2 H2 Scope Funs σ c Γ ->
+  Lemma Fun_inv_weak_in_Fun_inv k P1 P2 rho1 H1 rho2 H2 β Scope Funs σ c Γ :
+    Fun_inv k P1 P2 β rho1 H1 rho2 H2 Scope Funs σ c Γ ->
     Fun_inv_weak rho1 rho2 Scope Funs σ c Γ.
   Proof.
     intros HFun f v' Hnin Hin Hget.
     edestruct HFun as
         [vf [venv [Hnin' [Hget1 [Hget2 _]]]]]; eauto.
   Qed.
-
-  Lemma FV_inv_weak_in_FV_inv k P1 P2 rho1 H1 rho2 H2 Scope Funs c Γ FVs :
-    FV_inv k P1 P2 rho1 H1 rho2 H2 Scope Funs c Γ FVs ->
+  
+  Lemma FV_inv_weak_in_FV_inv k P1 P2 rho1 H1 rho2 H2 β Scope Funs c Γ FVs :
+    FV_inv k P1 P2 β rho1 H1 rho2 H2 Scope Funs c Γ FVs ->
     FV_inv_weak rho1 rho2 H2 Scope Funs c Γ FVs.
   Proof.
     intros HFV x N v' Hnin1 Hnin2 Hnth Hget.
     edestruct HFV as [vs [l' [v'' [Hget1 [Hget2 [Hnth' _]]]]]]; eauto.
     firstorder.
   Qed.
-
+  
   (** Correctness of [Closure_conversion] *)
   Lemma Closure_conversion_correct (k : nat) (H1 H2 : heap block)
         (rho1 rho2 : env) (e1 e2 : exp) (C : exp_ctx)
         (Scope Funs : Ensemble var) (FVs : list var)
-        (σ : var -> var) (c : cTag) (Γ : var) :
+        (σ : var -> var) (β : Inj) (c : cTag) (Γ : var) :
     (* [Scope] invariant *)
-    (H1, rho1) ⋞ ^ (Scope ; k ; IP Hole_c ; FP 0) (H2, rho2) ->
+    (forall j, (H1, rho1) ⋞ ^ (Scope ; k ; j ; IP k Hole_c ; FP 0 k H1 rho1 e1 ; β) (H2, rho2)) ->
     (* [Fun] invariant *)
-    Fun_inv k (IP Hole_c) (FP 0) rho1 H1 rho2 H2 Scope Funs σ c Γ ->
+    Fun_inv k (IP k Hole_c) (FP 0 k H1 rho1 e1) β rho1 H1 rho2 H2 Scope Funs σ c Γ ->
     (* Free variables invariant *)
-    FV_inv k (IP Hole_c) (FP 0) rho1 H1 rho2 H2 Scope Funs c Γ FVs ->
+    FV_inv k (IP k Hole_c) (FP 0 k H1 rho1 e1) β rho1 H1 rho2 H2 Scope Funs c Γ FVs ->
+    (* location renaming is injective *)
+    injective_subdomain (reach H1 (env_locs rho1 Scope)) β ->
 
+    
     (* well-formedness *)
     well_formed (reach' H1 (env_locs rho1 (occurs_free e1))) H1 ->
     (env_locs rho1 (occurs_free e1)) \subset dom H1 ->
@@ -255,30 +270,46 @@ Module ClosureConversionCorrect (H : Heap).
     (* function renaming codomain is not shadowed by other vars *)
     Disjoint _ (image σ (Setminus _ Funs Scope)) (bound_var e1) ->
 
+    
     (* [e'] is the closure conversion of [e] *)
     Closure_conversion clo_tag Scope Funs σ c Γ FVs e1 e2 C ->
-    (e1, rho1, H1) ⪯ ^ (k ; IP Hole_c ; IP Hole_c; FP 0 ; FP 0) (C |[ e2 ]|, rho2, H2).
+    
+    (forall j, (e1, rho1, H1) ⪯ ^ (k ; j ; IP k Hole_c ; IP k Hole_c; FP 0 k H1 rho1 e1 ; FP 0 k H1 rho1 e1) (C |[ e2 ]|, rho2, H2)).
   Proof with now eauto with Ensembles_DB.
-    revert H1 H2 rho1 rho2 e1 e2 C Scope Funs FVs σ c Γ.
+    revert H1 H2 rho1 rho2 e1 e2 C Scope Funs FVs σ β c Γ.
     induction k as [k IHk] using lt_wf_rec1.
-    intros H1 H2 rho1 rho2 e1 e2 C Scope Funs FVs σ c Γ
-           Henv Hfun HFVs Hwf1 Hlocs1 Hwf2 Hlos2 Hnin Hbind Hun Hinj Hd Hcc.
+    intros H1 H2 rho1 rho2 e1 e2 C Scope Funs FVs σ β c Γ
+           Henv Hfun HFVs Hinjb Hwf1 Hlocs1 Hwf2 Hlos2 Hnin Hbind Hun Hinj Hd Hcc.
     induction e1 using exp_ind'; try clear IHe1.
     - (* case Econstr *)
       inv Hcc.
-
+      
       edestruct (binding_in_map_getlist _ rho1 l Hbind) as [vl Hgetl].
       normalize_occurs_free...
-
+      
       edestruct project_vars_ctx_to_heap_env as [H2' [rho2' [m Hct]]]; try eassumption.
       eapply Fun_inv_weak_in_Fun_inv; eassumption.
       eapply FV_inv_weak_in_FV_inv; eassumption.
-      
-      eapply cc_approx_exp_right_ctx_compat;
-        [ exact FP_transfer | exact IP_ctx_to_heap_env | eassumption | eassumption
-        | eassumption | eassumption | eassumption | ]. 
 
-      eapply cc_approx_exp_constr_compat.
+      intros j. 
+      eapply cc_approx_exp_right_ctx_compat
+        with (ILi := fun c => FP c  k H1 rho1 (Econstr v t l e1));
+        [ now intros; eapply FP_transfer; eauto | now intros; eapply IP_ctx_to_heap_env; eauto
+          | eassumption | eassumption | eassumption | eassumption | eassumption | ].
+      rewrite <- plus_n_O.
+      eapply cc_approx_exp_constr_compat
+      with (ILi := fun c => FP c  k H1 rho1 (Econstr v t l e1));
+        [ | | | eassumption | | eassumption  | | | | ].
+      + admit. (* bounds *)
+      + admit. (* bounds *)
+      + admit. (* bounds *)
+      + admit. (* well_formed *)
+      + admit. (* env_locs *)
+      + admit. (* project_vars_correct *)
+      + admit. (* bounds *)
+      + (* Inductive case *)
+        intros i vs1 vs2 l1 l2 H1' H2'' Hlt Ha1 Ha2 Hall. (* bounds *)
+       
     - (* case Ecase nil *)
       inv Hcc.
       admit.
